specs/hmac_drbg_compspecs.v
@@ -1,0 +1,7 @@
+Require Import floyd.proofauto.
+Require Import hmac_drbg.
+
+Definition CompSpecs' : compspecs.
+Proof. make_compspecs1 prog. Defined.
+Instance CompSpecs : compspecs.
+Proof. make_compspecs2 CompSpecs'. Defined.
